IntMap.v
@@ -27,6 +27,11 @@ Definition IntMap_map {a b} (f : a -> b) (m : IntMap a) : IntMap b :=
   | getIntMap xs => getIntMap (map (fun x => (fst x, f (snd x))) xs)
   end.
 
+Definition IntMap_mergeWithKey {a b c} (combine : nat -> a -> b -> option c)
+  (only1 : IntMap a -> IntMap c) (only2 : IntMap b -> IntMap c)
+  (m1 : IntMap a) (m2 : IntMap b) : IntMap c :=
+  only1 m1.
+
 Definition IntMap_foldlWithKey
   {a b} (f : a -> nat -> b -> a) (z : a) (m : IntMap b) : a := z.
 
@@ -43,6 +48,7 @@ Extract Inlined Constant IntMap_insert       => "Data.IntMap.insert".
 Extract Inlined Constant IntMap_alter        => "Data.IntMap.alter".
 Extract Inlined Constant IntMap_map          => "Data.IntMap.map".
 Extract Inlined Constant IntMap_foldlWithKey => "Data.IntMap.foldlWithKey".
+Extract Inlined Constant IntMap_mergeWithKey => "Data.IntMap.mergeWithKey".
 Extract Inlined Constant IntMap_toList       => "Data.IntMap.toList".
 
 Inductive IntSet :=
